

Verifying the equations in Fermions as a non-local particle-hole excitation

Rishi Paresh Joshi

Our goal is to substitute $G_{\mathbf{k},a}$ (split into $G_{\mathbf{k}>}$ and $G_{\mathbf{k}<}$) into the given differential equations,

$$\begin{aligned} -\partial_\lambda G_{\mathbf{k}>}(\lambda, \lambda'; t, t') &= \sum_{\mathbf{p}} \frac{1}{e^{\beta(\epsilon_{\mathbf{k}} - \epsilon_{\mathbf{p}})} e^{\lambda + \lambda'} - 1} \left[e^{\lambda + \lambda'} e^{i(t-t')(\epsilon_{\mathbf{p}} - \epsilon_{\mathbf{k}})} G_{\mathbf{p}<}(\lambda, \lambda'; t, t') (1 - n_F(\mathbf{k})) \right. \\ &\quad \left. \times \left(\theta(t' - t) + \theta(t - t') e^{\beta(\epsilon_{\mathbf{k}} - \epsilon_{\mathbf{p}})} \right) - G_{\mathbf{k}>}(\lambda, \lambda'; t, t') n_F(\mathbf{p}) \right] \end{aligned} \quad (1)$$

and

$$\begin{aligned} -\partial_{\lambda'} G_{\mathbf{k}<}(\lambda, \lambda'; t, t') &= \sum_{\mathbf{p}} \frac{1}{e^{\beta(\epsilon_{\mathbf{p}} - \epsilon_{\mathbf{k}})} e^{\lambda + \lambda'} - 1} e^{i(t-t')(\epsilon_{\mathbf{p}} - \epsilon_{\mathbf{k}})} G_{\mathbf{p}>}(\lambda, \lambda'; t, t') n_F(\mathbf{k}) \\ &\quad \times \left(\theta(t - t') + e^{\beta(\epsilon_{\mathbf{p}} - \epsilon_{\mathbf{k}})} \theta(t' - t) \right) - G_{\mathbf{k}<}(\lambda, \lambda'; t, t') (1 - n_F(\mathbf{p})) \end{aligned} \quad (2)$$

and verify consistency.

1 Green's Functions we're provided with:

Let's define: $G_{\mathbf{k}>} = \tilde{G}_{\mathbf{k},>} e^{-i\epsilon_{\mathbf{k}}(t-t')}$ and $G_{\mathbf{p}<} = \tilde{G}_{\mathbf{p},<} e^{-i\epsilon_{\mathbf{p}}(t-t')}$.

Their expansion gives:

$$\tilde{G}_{\mathbf{k},>} = e^{\lambda'} \text{sgn}(t - t') \frac{(1 - n_F(\mathbf{k})) e^{\theta(t-t')\beta(\epsilon_{\mathbf{k}} - \mu)}}{1 + e^{\beta(\epsilon_{\mathbf{k}} - \mu)} e^{\lambda'}} \times \prod_{\mathbf{p}, n_F(\mathbf{p})=1} f_1(\lambda) \prod_{\mathbf{p}, n_F(\mathbf{p})=0} f_2(\lambda') \quad (3)$$

and,

$$\tilde{G}_{\mathbf{p},<} = \text{sgn}(t - t') \frac{n_F(\mathbf{p}) e^{-\theta(t'-t)\beta(\epsilon_{\mathbf{p}} - \mu)}}{1 + e^{-\beta(\epsilon_{\mathbf{p}} - \mu)} e^{\lambda}} \times \prod_{\mathbf{k}, n_F(\mathbf{k})=1} f_1(\lambda) \times \prod_{\mathbf{k}, n_F(\mathbf{k})=0} f_2(\lambda') \quad (4)$$

where: $f_1(\lambda) = \frac{e^{-\beta(\epsilon_{\mathbf{p}} - \mu)} + e^{-\lambda}}{1 + e^{-\beta(\epsilon_{\mathbf{p}} - \mu)}}$ and $f_2(\lambda') = \frac{e^{-\beta(\epsilon_{\mathbf{p}} - \mu)} e^{-\lambda'} + 1}{1 + e^{-\beta(\epsilon_{\mathbf{p}} - \mu)}}$.

We need to substitute these into the differential equation and test for equality. We have cancelled the $e^{-i\epsilon_{\mathbf{k}}(t-t')}$ term in the LHS and RHS. Eq.(1) becomes:

$$\begin{aligned} -\partial_\lambda \tilde{G}_{\mathbf{k}>}(\lambda, \lambda'; t, t') &= \sum_{\mathbf{p}} \frac{1}{e^{\beta(\epsilon_{\mathbf{k}} - \epsilon_{\mathbf{p}})} e^{\lambda + \lambda'} - 1} \left[e^{\lambda + \lambda'} \tilde{G}_{\mathbf{p}<}(\lambda, \lambda'; t, t') (1 - n_F(\mathbf{k})) \right. \\ &\quad \left. \times \left(\theta(t' - t) + \theta(t - t') e^{\beta(\epsilon_{\mathbf{k}} - \epsilon_{\mathbf{p}})} \right) - \tilde{G}_{\mathbf{k}>}(\lambda, \lambda'; t, t') n_F(\mathbf{p}) \right] \end{aligned} \quad (5)$$

Similarly, Eq.(2) becomes,

$$\begin{aligned} -\partial_{\lambda'} \tilde{G}_{\mathbf{k}<}(\lambda, \lambda'; t, t') &= \sum_{\mathbf{p}} \frac{1}{e^{\beta(\epsilon_{\mathbf{p}} - \epsilon_{\mathbf{k}})} e^{\lambda + \lambda'} - 1} \tilde{G}_{\mathbf{p}>}(\lambda, \lambda'; t, t') n_F(\mathbf{k}) \\ &\quad \times \left(\theta(t - t') + e^{\beta(\epsilon_{\mathbf{p}} - \epsilon_{\mathbf{k}})} \theta(t' - t) \right) - \tilde{G}_{\mathbf{k}<}(\lambda, \lambda'; t, t') (1 - n_F(\mathbf{p})) \end{aligned} \quad (6)$$

2 Verifying Eq.(1)

If we verify Eq.(5), then it means that we have verified Eq.(1).

2.1 Computing the Left-Hand Side of Eq.(5)

Substituting the given expressions for $\tilde{G}_{\mathbf{k},>}$ and $\tilde{G}_{\mathbf{p},<}$ into the left-hand side (LHS) of the differential equation provided. The LHS is $-\partial_\lambda \tilde{G}_{\mathbf{k},>}(\lambda, \lambda'; t, t')$, which requires us to compute the partial derivative of $\tilde{G}_{\mathbf{k},>}$ with respect to λ .

The expression for $\tilde{G}_{\mathbf{k},>}$ is from Eq.(3):

$$\tilde{G}_{\mathbf{k},>} = e^{\lambda'} \text{sgn}(t - t') \frac{(1 - n_F(\mathbf{k}))e^{\theta(t-t')\beta(\epsilon_{\mathbf{k}}-\mu)}}{1 + e^{\beta(\epsilon_{\mathbf{k}}-\mu)}e^{\lambda'}} \times \prod_{\mathbf{p}, n_F(\mathbf{p})=1} f_1(\lambda) \prod_{\mathbf{p}, n_F(\mathbf{p})=0} f_2(\lambda')$$

where:

$$f_1(\lambda) = \frac{e^{-\beta(\epsilon_{\mathbf{p}}-\mu)} + e^{-\lambda}}{1 + e^{-\beta(\epsilon_{\mathbf{p}}-\mu)}},$$

$$f_2(\lambda') = \frac{e^{-\beta(\epsilon_{\mathbf{p}}-\mu)}e^{-\lambda'} + 1}{1 + e^{-\beta(\epsilon_{\mathbf{p}}-\mu)}}.$$

This expression depends on both λ and λ' , and we need to compute its partial derivative with respect to λ . Note that λ appears in the product involving $f_1(\lambda)$, while λ' appears in the exponential factor $e^{\lambda'}$ and in the denominator of the fraction as well as in $f_2(\lambda')$.

Since $\tilde{G}_{\mathbf{k},>}$ is a product of terms, we apply the product rule for differentiation. Let us denote the expression as:

$$\tilde{G}_{\mathbf{k},>} = A \cdot B \cdot C$$

where:

$$A = e^{\lambda'} \text{sgn}(t - t') \frac{(1 - n_F(\mathbf{k}))e^{\theta(t-t')\beta(\epsilon_{\mathbf{k}}-\mu)}}{1 + e^{\beta(\epsilon_{\mathbf{k}}-\mu)}e^{\lambda'}},$$

$$B = \prod_{\mathbf{p}, n_F(\mathbf{p})=1} f_1(\lambda),$$

$$C = \prod_{\mathbf{p}, n_F(\mathbf{p})=0} f_2(\lambda').$$

The partial derivative with respect to λ is:

$$\partial_\lambda \tilde{G}_{\mathbf{k},>} = (\partial_\lambda A) \cdot B \cdot C + A \cdot (\partial_\lambda B) \cdot C + A \cdot B \cdot (\partial_\lambda C)$$

Term 1: $\partial_\lambda A$

A does not depend on λ (since λ appears only in $f_1(\lambda)$, which is in B), so:

$$\partial_\lambda A = 0$$

Term 2: $\partial_\lambda C$

$C = \prod_{\mathbf{p}, n_F(\mathbf{p})=0} f_2(\lambda')$ depends only on λ' , not λ , so:

$$\partial_\lambda C = 0$$

Term 3: $\partial_\lambda B$

$B = \prod_{\mathbf{p}, n_F(\mathbf{p})=1} f_1(\lambda)$. For a product, the derivative is:

$$\partial_\lambda B = \sum_{\mathbf{p}, n_F(\mathbf{p})=1} (\partial_\lambda f_1(\lambda)) \prod_{\mathbf{q} \neq \mathbf{p}, n_F(\mathbf{q})=1} f_1(\lambda)$$

Now, we compute $\partial_\lambda f_1(\lambda)$:

$$f_1(\lambda) = \frac{e^{-\beta(\epsilon_{\mathbf{p}}-\mu)} + e^{-\lambda}}{1 + e^{-\beta(\epsilon_{\mathbf{p}}-\mu)}}$$

The denominator is constant with respect to λ , so:

$$\partial_\lambda f_1(\lambda) = \frac{\partial_\lambda (e^{-\beta(\epsilon_{\mathbf{p}}-\mu)} + e^{-\lambda})}{1 + e^{-\beta(\epsilon_{\mathbf{p}}-\mu)}} = \frac{0 + (-e^{-\lambda})}{1 + e^{-\beta(\epsilon_{\mathbf{p}}-\mu)}} = -\frac{e^{-\lambda}}{1 + e^{-\beta(\epsilon_{\mathbf{p}}-\mu)}}$$

Thus:

$$\partial_\lambda B = \sum_{\mathbf{p}, n_F(\mathbf{p})=1} \left(-\frac{e^{-\lambda}}{1 + e^{-\beta(\epsilon_{\mathbf{p}} - \mu)}} \right) \prod_{\mathbf{q} \neq \mathbf{p}, n_F(\mathbf{q})=1} f_1(\lambda)$$

Therefore:

$$\begin{aligned} \partial_\lambda \tilde{G}_{\mathbf{k}, >} &= A \cdot \left(\sum_{\mathbf{p}, n_F(\mathbf{p})=1} \left(-\frac{e^{-\lambda}}{1 + e^{-\beta(\epsilon_{\mathbf{p}} - \mu)}} \right) \prod_{\mathbf{q} \neq \mathbf{p}, n_F(\mathbf{q})=1} f_1(\lambda) \right) \cdot C \\ -\partial_\lambda \tilde{G}_{\mathbf{k}, >} &= -A \cdot C \cdot \sum_{\mathbf{p}, n_F(\mathbf{p})=1} \left(-\frac{e^{-\lambda}}{1 + e^{-\beta(\epsilon_{\mathbf{p}} - \mu)}} \right) \prod_{\mathbf{q} \neq \mathbf{p}, n_F(\mathbf{q})=1} f_1(\lambda) \\ &= A \cdot C \cdot \sum_{\mathbf{p}, n_F(\mathbf{p})=1} \frac{e^{-\lambda}}{1 + e^{-\beta(\epsilon_{\mathbf{p}} - \mu)}} \prod_{\mathbf{q} \neq \mathbf{p}, n_F(\mathbf{q})=1} f_1(\lambda) \end{aligned}$$

Multiplying and dividing by $f_1(\lambda) = \frac{e^{-\beta(\epsilon_{\mathbf{p}} - \mu)} + e^{-\lambda}}{1 + e^{-\beta(\epsilon_{\mathbf{p}} - \mu)}}$ to make the product over all \mathbf{q} ,

$$-\partial_\lambda \tilde{G}_{\mathbf{k}, >} = A \cdot C \cdot \sum_{\mathbf{p}, n_F(\mathbf{p})=1} \left(\frac{e^{-\lambda}}{e^{-\beta(\epsilon_{\mathbf{p}} - \mu)} + e^{-\lambda}} \right) \prod_{\mathbf{q}, n_F(\mathbf{q})=1} f_1(\lambda)$$

Substituting A and C :

$$-\partial_\lambda \tilde{G}_{\mathbf{k}, >} = \left(e^{\lambda'} \text{sgn}(t - t') \frac{(1 - n_F(\mathbf{k})) e^{\theta(t - t')\beta(\epsilon_{\mathbf{k}} - \mu)}}{1 + e^{\beta(\epsilon_{\mathbf{k}} - \mu)} e^{\lambda'}} \right) \cdot \left(\prod_{\mathbf{p}, n_F(\mathbf{p})=0} f_2(\lambda') \right) \cdot \sum_{\mathbf{p}, n_F(\mathbf{p})=1} \left(\frac{e^{-\lambda}}{e^{-\beta(\epsilon_{\mathbf{p}} - \mu)} + e^{-\lambda}} \right) \prod_{\mathbf{q}, n_F(\mathbf{q})=1} f_1(\lambda)$$

Substitution into the LHS

The LHS of the differential equation is $-\partial_\lambda \tilde{G}_{\mathbf{k}, >}(\lambda, \lambda'; t, t')$, so the above result is the substituted form. The expression is as follows: as follows:

$$\begin{aligned} -\partial_\lambda \tilde{G}_{\mathbf{k}, >} &= \sum_{\mathbf{p}, n_F(\mathbf{p})=1} \left(\frac{e^{-\lambda}}{e^{-\beta(\epsilon_{\mathbf{p}} - \mu)} + e^{-\lambda}} \right) e^{\lambda'} \text{sgn}(t - t') \frac{(1 - n_F(\mathbf{k})) e^{\theta(t - t')\beta(\epsilon_{\mathbf{k}} - \mu)}}{1 + e^{\beta(\epsilon_{\mathbf{k}} - \mu)} e^{\lambda'}} \cdot \prod_{\mathbf{q}, n_F(\mathbf{q})=0} f_2(\lambda') \cdot \prod_{\mathbf{q}, n_F(\mathbf{q})=1} f_1(\lambda) \\ &= \sum_{\mathbf{p}, n_F(\mathbf{p})=1} \left(\frac{e^{-\lambda}}{e^{-\beta(\epsilon_{\mathbf{p}} - \mu)} + e^{-\lambda}} \right) \tilde{G}_{\mathbf{k}, >} \end{aligned}$$

2.2 Computing the Right-Hand Side of Eq.(5)

The RHS of Eq.(5) is given by:

$$\sum_{\mathbf{p}} \frac{1}{e^{\beta(\epsilon_{\mathbf{k}} - \epsilon_{\mathbf{p}})} e^{\lambda + \lambda'} - 1} \left[e^{\lambda + \lambda'} \tilde{G}_{\mathbf{p} <}(\lambda, \lambda'; t, t') (1 - n_F(\mathbf{k})) \times \left(\theta(t' - t) + \theta(t - t') e^{\beta(\epsilon_{\mathbf{k}} - \epsilon_{\mathbf{p}})} \right) - \tilde{G}_{\mathbf{k} >}(\lambda, \lambda'; t, t') n_F(\mathbf{p}) \right]$$

This means that the sum is implicitly over $n_F(\mathbf{p}) = 1$.

$$RHS = \sum_{\mathbf{p}, n_F(\mathbf{p})=1} \frac{1}{e^{\beta(\epsilon_{\mathbf{k}} - \epsilon_{\mathbf{p}})} e^{\lambda + \lambda'} - 1} \left[e^{\lambda + \lambda'} \tilde{G}_{\mathbf{p} <}(\lambda, \lambda'; t, t') (1 - n_F(\mathbf{k})) \times \left(\theta(t' - t) + \theta(t - t') e^{\beta(\epsilon_{\mathbf{k}} - \epsilon_{\mathbf{p}})} \right) - \tilde{G}_{\mathbf{k} >}(\lambda, \lambda'; t, t') \right]$$

We summarize a couple of things we noticed:

- $(1 - n_F(\mathbf{k})) = 1$ and $n_F(\mathbf{p}) = 1$ are in both LHS and RHS. Hence, we need to check only when these conditions are met.
- We get a summation over \mathbf{p} in LHS after taking the derivative, and we had a summation over \mathbf{p} in RHS before. If these match term by term, our result is verified. If not we will have to struggle.

We take the cases,

2.2.1 Case 1: t' is greater than t

$$\begin{aligned} RHS &= \sum_{\mathbf{p}, n_F(\mathbf{p})=1} \frac{1}{e^{\beta(\epsilon_{\mathbf{k}} - \epsilon_{\mathbf{p}})} e^{\lambda + \lambda'} - 1} \left[e^{\lambda + \lambda'} \tilde{G}_{\mathbf{p} <}(\lambda, \lambda'; t, t') (1 - n_F(\mathbf{k})) - \tilde{G}_{\mathbf{k} >}(\lambda, \lambda'; t, t') \right] \\ &= \sum_{\mathbf{p}, n_F(\mathbf{p})=1} \frac{(1 - n_F(\mathbf{k}))}{e^{\beta(\epsilon_{\mathbf{k}} - \epsilon_{\mathbf{p}})} e^{\lambda + \lambda'} - 1} \left[-\frac{e^{\lambda + \lambda'} e^{-\beta(\epsilon_{\mathbf{p}} - \mu)}}{1 + e^{-\beta(\epsilon_{\mathbf{p}} - \mu)} e^{\lambda}} + \frac{e^{\lambda'}}{1 + e^{\beta(\epsilon_{\mathbf{k}} - \mu)} e^{\lambda'}} \right] \times \prod_{\mathbf{q}, n_F(\mathbf{q})=1} f_1(\lambda) \times \prod_{\mathbf{q}, n_F(\mathbf{q})=0} f_2(\lambda') \end{aligned}$$

Using mathematical, we find that,

$$\begin{aligned} &\frac{1}{e^{\beta(\epsilon_{\mathbf{k}} - \epsilon_{\mathbf{p}})} e^{\lambda + \lambda'} - 1} \left[-\frac{e^{\lambda + \lambda'} e^{-\beta(\epsilon_{\mathbf{p}} - \mu)}}{1 + e^{-\beta(\epsilon_{\mathbf{p}} - \mu)} e^{\lambda}} + \frac{e^{\lambda'}}{1 + e^{\beta(\epsilon_{\mathbf{k}} - \mu)} e^{\lambda'}} \right] \\ &= - \left(\frac{e^{-\lambda}}{e^{-\beta(\epsilon_{\mathbf{p}} - \mu)} + e^{-\lambda}} \right) \times \frac{e^{\lambda'}}{1 + e^{\beta(\epsilon_{\mathbf{k}} - \mu)} e^{\lambda'}} \end{aligned}$$

which is on the LHS when $t' > t$. Thus, the summation matches term by term.

Interesting question: Would we require this term-by-term matching condition, and can it also be related to creating local equations that may be simpler to solve?

2.2.2 Case 2: t' is lesser than t

$$\begin{aligned} RHS &= \sum_{\mathbf{p}, n_F(\mathbf{p})=1} \frac{(1 - n_F(\mathbf{k}))}{e^{\beta(\epsilon_{\mathbf{k}} - \epsilon_{\mathbf{p}})} e^{\lambda + \lambda'} - 1} \left[e^{\lambda + \lambda'} e^{\beta(\epsilon_{\mathbf{k}} - \epsilon_{\mathbf{p}})} \tilde{G}_{\mathbf{p} <}(\lambda, \lambda'; t, t') - \tilde{G}_{\mathbf{k} >}(\lambda, \lambda'; t, t') \right] \\ RHS &= \sum_{\mathbf{p}, n_F(\mathbf{p})=1} \frac{(1 - n_F(\mathbf{k}))}{e^{\beta(\epsilon_{\mathbf{k}} - \epsilon_{\mathbf{p}})} e^{\lambda + \lambda'} - 1} \left[\frac{e^{\lambda + \lambda'} e^{\beta(\epsilon_{\mathbf{k}} - \epsilon_{\mathbf{p}})}}{1 + e^{-\beta(\epsilon_{\mathbf{p}} - \mu)} e^{\lambda}} - \frac{e^{\lambda'} e^{\beta(\epsilon_{\mathbf{k}} - \mu)}}{1 + e^{\beta(\epsilon_{\mathbf{k}} - \mu)} e^{\lambda'}} \right] \times \prod_{\mathbf{k}, n_F(\mathbf{k})=1} f_1(\lambda) \times \prod_{\mathbf{k}, n_F(\mathbf{k})=0} f_2(\lambda') \end{aligned}$$

Using Mathematica, we find that:

$$\begin{aligned} &\frac{1}{e^{\beta(\epsilon_{\mathbf{k}} - \epsilon_{\mathbf{p}})} e^{\lambda + \lambda'} - 1} \left[\frac{e^{\lambda + \lambda'} e^{\beta(\epsilon_{\mathbf{k}} - \epsilon_{\mathbf{p}})}}{1 + e^{-\beta(\epsilon_{\mathbf{p}} - \mu)} e^{\lambda}} - \frac{e^{\lambda'} e^{\beta(\epsilon_{\mathbf{k}} - \mu)}}{1 + e^{\beta(\epsilon_{\mathbf{k}} - \mu)} e^{\lambda'}} \right] \\ &= \left(\frac{e^{-\lambda}}{e^{-\beta(\epsilon_{\mathbf{p}} - \mu)} + e^{-\lambda}} \right) \times \frac{e^{\lambda'} e^{\beta(\epsilon_{\mathbf{k}} - \mu)}}{1 + e^{\beta(\epsilon_{\mathbf{k}} - \mu)} e^{\lambda'}} \end{aligned}$$

3 Verifying Eq.(2)

If we verify Eq.(6), then it means that we have verified Eq.(2)

3.1 Computing the Left-Hand side of Eq.(6)

Substituting the given expressions for $\tilde{G}_{\mathbf{p}, >}$ and $\tilde{G}_{\mathbf{k}, <}$ into the left-hand side (LHS) of the differential equation provided. The LHS is $-\partial_{\lambda'} \tilde{G}_{\mathbf{k}, <}(\lambda, \lambda'; t, t')$, which requires us to compute the partial derivative of $\tilde{G}_{\mathbf{k}, <}$ with respect to λ . The expression for $\tilde{G}_{\mathbf{k}, <}$ is from Eq.(4):

$$\tilde{G}_{\mathbf{k}, <} = \text{sgn}(t - t') \frac{n_F(\mathbf{k}) e^{-\theta(t' - t)\beta(\epsilon_{\mathbf{k}} - \mu)}}{1 + e^{-\beta(\epsilon_{\mathbf{k}} - \mu)} e^{\lambda}} \times \prod_{\mathbf{p}, n_F(\mathbf{p})=1} f_1(\lambda) \times \prod_{\mathbf{p}, n_F(\mathbf{p})=0} f_2(\lambda')$$

where:

$$f_1(\lambda) = \frac{e^{-\beta(\epsilon_{\mathbf{p}} - \mu)} + e^{-\lambda}}{1 + e^{-\beta(\epsilon_{\mathbf{p}} - \mu)}},$$

$$f_2(\lambda') = \frac{e^{-\beta(\epsilon_{\mathbf{p}} - \mu)} e^{-\lambda'} + 1}{1 + e^{-\beta(\epsilon_{\mathbf{p}} - \mu)}}.$$

To compute the partial derivative $-\partial_{\lambda'} \tilde{G}_{\mathbf{k}, <}(\lambda, \lambda'; t, t')$, we begin by carefully analyzing the given expression for $\tilde{G}_{\mathbf{k}, <}$. The expression is a product of three distinct factors, and we must determine how each depends on the variable λ' to apply the product rule for differentiation correctly. Let us denote the expression as:

$$\tilde{G}_{\mathbf{k},<} = A \times B \times C,$$

where:

$$1. A = \text{sgn}(t - t') \frac{n_F(\mathbf{k}) e^{-\theta(t' - t)\beta(\epsilon_{\mathbf{k}} - \mu)}}{1 + e^{-\beta(\epsilon_{\mathbf{k}} - \mu)} e^\lambda},$$

$$2. B = \prod_{\mathbf{p}, n_F(\mathbf{p})=1} f_1(\lambda),$$

$$3. C = \prod_{\mathbf{p}, n_F(\mathbf{p})=0} f_2(\lambda'),$$

$$\text{with the functions defined as: } f_1(\lambda) = \frac{e^{-\beta(\epsilon_{\mathbf{p}} - \mu)} + e^{-\lambda}}{1 + e^{-\beta(\epsilon_{\mathbf{p}} - \mu)}},$$

$$f_2(\lambda') = \frac{e^{-\beta(\epsilon_{\mathbf{p}} - \mu)} e^{-\lambda'} + 1}{1 + e^{-\beta(\epsilon_{\mathbf{p}} - \mu)}}.$$

The goal is to compute $-\frac{\partial}{\partial \lambda'} \tilde{G}_{\mathbf{k},<}$, where $\tilde{G}_{\mathbf{k},<}$ depends on both λ and λ' , as well as t and t' . Since this is a partial derivative with respect to λ' , we treat λ , t , and t' as constants.

Factor A : This term depends on λ , t , t' , and various parameters (β , $\epsilon_{\mathbf{k}}$, μ , etc.), but it contains no λ' . Thus, $\frac{\partial A}{\partial \lambda'} = 0$.

Factor B : The product involves $f_1(\lambda)$, which depends only on λ and not on λ' . Hence, $\frac{\partial B}{\partial \lambda'} = 0$.

Factor C : This is a product over \mathbf{p} where $n_F(\mathbf{k}) = 0$, and each $f_2(\lambda')$ explicitly depends on λ' . Therefore, the derivative will act solely on this factor.

Since A and B are independent of λ' , the partial derivative of the product simplifies to:

$$\frac{\partial}{\partial \lambda'} (A \cdot B \cdot C) = A \cdot B \cdot \frac{\partial C}{\partial \lambda'},$$

where A and B are treated as constants with respect to λ' . Thus:

$$-\frac{\partial}{\partial \lambda'} \tilde{G}_{\mathbf{k},<} = -A \cdot B \cdot \frac{\partial C}{\partial \lambda'}.$$

The factor C is a product:

$$C = \prod_{\mathbf{p}, n_F(\mathbf{p})=0} f_2(\lambda'),$$

where $f_2(\lambda') = \frac{e^{-\beta(\epsilon_{\mathbf{p}} - \mu)} e^{-\lambda'} + 1}{1 + e^{-\beta(\epsilon_{\mathbf{p}} - \mu)}}$. For a product of functions $\prod_i g_i(x)$, the derivative is:

$$\frac{\partial}{\partial x} \prod_i g_i(x) = \left(\prod_i g_i(x) \right) \sum_i \frac{g'_i(x)}{g_i(x)}.$$

Here, $g_i = f_2(\lambda')$ for each \mathbf{p} in the set where $n_F(\mathbf{k}) = 0$. We need to compute the logarithmic derivative $\frac{f'_2(\lambda')}{f_2(\lambda')}$.

Let the numerator of $f_2(\lambda')$ be $N = e^{-\beta(\epsilon_{\mathbf{p}} - \mu)} e^{-\lambda'} + 1$ and the denominator be $D = 1 + e^{-\beta(\epsilon_{\mathbf{p}} - \mu)}$, so $f_2(\lambda') = \frac{N}{D}$. Since D is constant with respect to λ' :

$$\frac{\partial f_2}{\partial \lambda'} = \frac{1}{D} \frac{\partial N}{\partial \lambda'}.$$

Now, compute:

$$\frac{\partial N}{\partial \lambda'} = \frac{\partial}{\partial \lambda'} \left(e^{-\beta(\epsilon_{\mathbf{p}} - \mu)} e^{-\lambda'} + 1 \right) = e^{-\beta(\epsilon_{\mathbf{p}} - \mu)} \cdot (-e^{-\lambda'}) = -e^{-\beta(\epsilon_{\mathbf{p}} - \mu)} e^{-\lambda'},$$

since the derivative of $e^{-\lambda'} = -e^{-\lambda'}$ and the constant term 1 has derivative zero. Thus:

$$\frac{\partial f_2}{\partial \lambda'} = \frac{-e^{-\beta(\epsilon_{\mathbf{p}} - \mu)} e^{-\lambda'}}{1 + e^{-\beta(\epsilon_{\mathbf{p}} - \mu)}}.$$

Logarithmic Derivative:

$$\frac{\frac{\partial f_2}{\partial \lambda'}}{f_2(\lambda')} = \frac{-\frac{e^{-\beta(\epsilon_{\mathbf{p}} - \mu)} e^{-\lambda'}}{1 + e^{-\beta(\epsilon_{\mathbf{p}} - \mu)}}}{\frac{e^{-\beta(\epsilon_{\mathbf{p}} - \mu)} e^{-\lambda'} + 1}{1 + e^{-\beta(\epsilon_{\mathbf{p}} - \mu)}}} = -\frac{e^{-\beta(\epsilon_{\mathbf{p}} - \mu)} e^{-\lambda'}}{e^{-\beta(\epsilon_{\mathbf{p}} - \mu)} e^{-\lambda'} + 1}.$$

For the product C :

$$\frac{\partial C}{\partial \lambda'} = C \sum_{\mathbf{p}, n_F(\mathbf{p})=0} \frac{\frac{\partial f_2}{\partial \lambda'}}{f_2(\lambda')} = C \sum_{\mathbf{p}, n_F(\mathbf{p})=0} \left(-\frac{e^{-\beta(\epsilon_{\mathbf{p}}-\mu)} e^{-\lambda'}}{e^{-\beta(\epsilon_{\mathbf{p}}-\mu)} e^{-\lambda'} + 1} \right).$$

Substituting back gives us:

$$-\frac{\partial}{\partial \lambda'} \tilde{G}_{\mathbf{k},<} = -A \cdot B \cdot \frac{\partial C}{\partial \lambda'} = -A \cdot B \cdot C \sum_{\mathbf{p}, n_F(\mathbf{p})=0} \left(-\frac{e^{-\beta(\epsilon_{\mathbf{p}}-\mu)} e^{-\lambda'}}{e^{-\beta(\epsilon_{\mathbf{p}}-\mu)} e^{-\lambda'} + 1} \right).$$

The two negatives on the RHS of the above equation cancel, yielding:

$$-\frac{\partial}{\partial \lambda'} \tilde{G}_{\mathbf{k},<} = (A \cdot B \cdot C) \sum_{\mathbf{p}, n_F(\mathbf{p})=0} \frac{e^{-\beta(\epsilon_{\mathbf{p}}-\mu)} e^{-\lambda'}}{e^{-\beta(\epsilon_{\mathbf{p}}-\mu)} e^{-\lambda'} + 1}.$$

Since $A \cdot B \cdot C = \tilde{G}_{\mathbf{k},<}$, the final result is:

$$-\frac{\partial}{\partial \lambda'} \tilde{G}_{\mathbf{k},<}(\lambda, \lambda'; t, t') = \tilde{G}_{\mathbf{k},<}(\lambda, \lambda'; t, t') \sum_{\mathbf{p}, n_F(\mathbf{p})=0} \frac{e^{-\beta(\epsilon_{\mathbf{p}}-\mu)} e^{-\lambda'}}{e^{-\beta(\epsilon_{\mathbf{p}}-\mu)} e^{-\lambda'} + 1}.$$

3.2 Computing the Right-Hand Side of Eq.(6)

The RHS of Eq.(6) is given by:

$$\sum_{\mathbf{p}} \frac{1}{e^{\beta(\epsilon_{\mathbf{p}}-\epsilon_{\mathbf{k}})} e^{\lambda+\lambda'} - 1} \left[\tilde{G}_{\mathbf{p}>}(\lambda, \lambda'; t, t') n_F(\mathbf{k}) \times \left(\theta(t-t') + e^{\beta(\epsilon_{\mathbf{p}}-\epsilon_{\mathbf{k}})} \theta(t'-t) \right) - \tilde{G}_{\mathbf{k}<}(\lambda, \lambda'; t, t') (1 - n_F(\mathbf{p})) \right]$$

This means that the sum is implicitly over $n_F(\mathbf{p}) = 0$

$$RHS = \sum_{\mathbf{p}, n_F(\mathbf{p})=0} \frac{1}{e^{\beta(\epsilon_{\mathbf{p}}-\epsilon_{\mathbf{k}})} e^{\lambda+\lambda'} - 1} \left[\tilde{G}_{\mathbf{p}>}(\lambda, \lambda'; t, t') n_F(\mathbf{k}) \times \left(\theta(t-t') + e^{\beta(\epsilon_{\mathbf{p}}-\epsilon_{\mathbf{k}})} \theta(t'-t) \right) - \tilde{G}_{\mathbf{k}<}(\lambda, \lambda'; t, t') \right]$$

Using,

$$\tilde{G}_{\mathbf{p},>} = e^{\lambda'} \text{sgn}(t-t') \frac{(1 - n_F(\mathbf{p})) e^{\theta(t-t')\beta(\epsilon_{\mathbf{p}}-\mu)}}{1 + e^{\beta(\epsilon_{\mathbf{p}}-\mu)} e^{\lambda'}} \times \prod_{\mathbf{q}, n_F(\mathbf{q})=1} f_1(\lambda) \prod_{\mathbf{q}, n_F(\mathbf{q})=0} f_2(\lambda')$$

and

$$\tilde{G}_{\mathbf{k},<} = \text{sgn}(t-t') \frac{n_F(\mathbf{k}) e^{-\theta(t'-t)\beta(\epsilon_{\mathbf{k}}-\mu)}}{1 + e^{-\beta(\epsilon_{\mathbf{k}}-\mu)} e^{\lambda}} \times \prod_{\mathbf{q}, n_F(\mathbf{q})=1} f_1(\lambda) \times \prod_{\mathbf{q}, n_F(\mathbf{q})=0} f_2(\lambda')$$

where:

$$f_1(\lambda) = \frac{e^{-\beta(\epsilon_{\mathbf{q}}-\mu)} + e^{-\lambda}}{1 + e^{-\beta(\epsilon_{\mathbf{q}}-\mu)}},$$

$$f_2(\lambda') = \frac{e^{-\beta(\epsilon_{\mathbf{q}}-\mu)} e^{-\lambda'} + 1}{1 + e^{-\beta(\epsilon_{\mathbf{q}}-\mu)}}$$

3.2.1 Case 1: t' is greater than t

$$RHS = \sum_{\mathbf{p}, n_F(\mathbf{p})=0} \frac{1}{e^{\beta(\epsilon_{\mathbf{p}}-\epsilon_{\mathbf{k}})} e^{\lambda+\lambda'} - 1} \left[\frac{-e^{\lambda'} e^{\beta(\epsilon_{\mathbf{p}}-\epsilon_{\mathbf{k}})}}{1 + e^{\beta(\epsilon_{\mathbf{p}}-\mu)} e^{\lambda'}} n_F(\mathbf{k}) + \frac{n_F(\mathbf{k}) e^{-\beta(\epsilon_{\mathbf{k}}-\mu)}}{1 + e^{-\beta(\epsilon_{\mathbf{k}}-\mu)} e^{\lambda}} \right] \times \prod_{\mathbf{q}, n_F(\mathbf{q})=1} f_1(\lambda) \prod_{\mathbf{q}, n_F(\mathbf{q})=0} f_2(\lambda')$$

Or,

$$RHS = \tilde{G}_{\mathbf{k},<} \sum_{\mathbf{p}, n_F(\mathbf{p})=0} \frac{1}{e^{\beta(\epsilon_{\mathbf{p}}-\epsilon_{\mathbf{k}})} e^{\lambda+\lambda'} - 1} \left[\frac{-e^{\lambda'} e^{\beta(\epsilon_{\mathbf{p}}-\epsilon_{\mathbf{k}})} (1 + e^{-\beta(\epsilon_{\mathbf{k}}-\mu)} e^{\lambda})}{(1 + e^{\beta(\epsilon_{\mathbf{p}}-\mu)} e^{\lambda'}) e^{-\beta(\epsilon_{\mathbf{k}}-\mu)}} + 1 \right]$$

This is equal to the LHS, when simplified on Mathematica.

3.2.2 Case 2: t' is lesser than t

$$\begin{aligned}
RHS &= \sum_{\mathbf{p}, n_F(\mathbf{p})=0} \frac{1}{e^{\beta(\epsilon_{\mathbf{p}}-\epsilon_{\mathbf{k}})} e^{\lambda+\lambda'} - 1} \left[e^{\lambda'} \frac{(1 - n_F(\mathbf{p})) e^{\beta(\epsilon_{\mathbf{p}}-\mu)}}{1 + e^{\beta(\epsilon_{\mathbf{p}}-\mu)} e^{\lambda'}} n_F(\mathbf{k}) - \frac{n_F(\mathbf{k})}{1 + e^{-\beta(\epsilon_{\mathbf{k}}-\mu)} e^{\lambda}} \right] \times \prod_{\mathbf{q}, n_F(\mathbf{q})=1} f_1(\lambda) \times \prod_{\mathbf{q}, n_F(\mathbf{q})=0} f_2(\lambda') \\
RHS &= \tilde{G}_{\mathbf{k}, <} \sum_{\mathbf{p}, n_F(\mathbf{p})=0} \frac{1}{e^{\beta(\epsilon_{\mathbf{p}}-\epsilon_{\mathbf{k}})} e^{\lambda+\lambda'} - 1} \left[\frac{e^{\lambda'} e^{\beta(\epsilon_{\mathbf{p}}-\mu)} (1 + e^{-\beta(\epsilon_{\mathbf{k}}-\mu)} e^{\lambda})}{1 + e^{\beta(\epsilon_{\mathbf{p}}-\mu)} e^{\lambda'}} - 1 \right]
\end{aligned}$$

This, too, is equal to the LHS when simplified on Mathematica.